\documentclass[10pt,twocolumn,twoside,a4paper]{article}
\usepackage[margin=0.6in]{geometry}
\usepackage{algorithm}
\usepackage{multicol}
\usepackage{algorithmic}
\usepackage{amsmath}
\usepackage{bm}
\usepackage{blindtext}
\usepackage{amsfonts}
\usepackage{multirow}
\usepackage{graphicx}
\begin{document}
\title{EECS487 Lab0}
\author{Xiaofei Wang 56209720}
\maketitle
\section*{Angle Between Vectors}
Denote the angle by $\alpha(\vec{u}, \vec{v})$. We have
\begin{align*}
\text{cos}\alpha(\vec{u}, \vec{v})
&=\frac{\left\langle\vec{u}, \vec{v}\right\rangle}{||\vec{u}||\cdot||\vec{v}||}\\
&=\frac{1\times(-5)+2\times8+3\times(-2)}{\sqrt{(1^2+2^2+3^2)((-5)^2+8^2+(-2)^2)}}\\
&=\frac{5}{\sqrt{1302}}
\end{align*}
Therefore $\alpha(\vec{u}, \vec{v})=\text{arccos}\frac{5}{\sqrt{1302}}\approx1.43\text{rad}=82.035\text{degree}$
\section*{Linear Equations With Matrices}
The equations can be denoted by
\[
\left(
\begin{array}{ccc}
2&6&2\\
1&9&3\\
-3&-3&1
\end{array}
\right)
\left(
\begin{array}{c}
x\\
y\\
z
\end{array}
\right)
=\left(
\begin{array}{c}
-2\\
1\\
-1
\end{array}
\right)
\]
We have
\[
\left(
\begin{array}{c}
x\\
y\\
z
\end{array}
\right)=\left(
\begin{array}{ccc}
2&6&2\\
1&9&3\\
-3&-3&1
\end{array}
\right)^{-1}\left(
\begin{array}{c}
-2\\
1\\
-1
\end{array}
\right)
\]
denote
\[
A=\left(
\begin{array}{ccc}
2&6&2\\
1&9&3\\
-3&-3&1
\end{array}
\right)
\]
and $\text{Cof}A$ the cofactor of $A$. We have
\[
A^{-1}=\frac{1}{\text{det}A}(\text{Cof}A)^T
\]
\[
\text{det}A=2\times(9+9)-1\times(6+6)-3\times(18-18)=24
\]
\begin{align*}
\text{Cof}A\\
&=\left(
\begin{array}{ccc}
9+9&-(1+9)&-3+27\\
-(6+6)&2+6&-(-6+18)\\
18-18&-(6-2)&18-6
\end{array}
\right)\\
&=\left(
\begin{array}{ccc}
18&-10&24\\
-12&8&-12\\
0&-4&12
\end{array}
\right)
\end{align*}
\[
\text{Cof}A^T=\left(
\begin{array}{ccc}
18&-12&0\\
-10&8&-4\\
24&-12&12
\end{array}
\right)\\
\]
\begin{align*}
A^{-1}&=\frac{1}{\text{det}A}(\text{Cof}A)^T\\
&=\left(
\begin{array}{ccc}
\frac{3}{4}&-\frac{1}{2}&0\\
-\frac{5}{12}&\frac{1}{3}&-\frac{1}{6}\\
1&-\frac{1}{2}&\frac{1}{2}
\end{array}
\right)
\end{align*}
Therefore 
\begin{align*}
\left(
\begin{array}{c}
x\\
y\\
z
\end{array}
\right)&=\left(
\begin{array}{ccc}
\frac{3}{4}&-\frac{1}{2}&0\\
-\frac{5}{12}&\frac{1}{3}&-\frac{1}{6}\\
1&-\frac{1}{2}&\frac{1}{2}
\end{array}
\right)\left(
\begin{array}{c}
-2\\
1\\
-1
\end{array}
\right)\\
&=\left(
\begin{array}{c}
-\frac{3}{2}-\frac{1}{2}+0\\
\frac{5}{6}+\frac{1}{3}+\frac{1}{6}\\
-2-\frac{1}{2}-\frac{1}{2}
\end{array}
\right)\\
&=\left(
\begin{array}{c}
-2\\
\frac{4}{3}\\
-3
\end{array}
\right)
\end{align*}
\section*{Projection}
The component of $\vec{u}$ orthogonal to $\vec{v}$ is $\vec{u}-\frac{\vec{v}}{||\vec{v}||^2}(\vec{u}\cdot\vec{v})$.
\begin{align*}
\vec{u}-\frac{\vec{v}}{||\vec{v}||^2}(\vec{u}\cdot\vec{v})&=\left\langle-3,2,4\right\rangle+\frac{10}{5}\left\langle2,0,-1\right\rangle\\
&=\left\langle1,2,2\right\rangle
\end{align*}
\section*{Triangle Area}
\[
S=\frac{1}{2}||\vec{u}\times\vec{v}||=\frac{3\sqrt{5}}{2} 
\]
\section*{Matrix Multiplication}
\begin{align*}
\hat M\hat N
&=\left(
\begin{array}{ccc}
-5+21-18&6+35-12&10-49-6\\
-10+6-24&12+10-16&20-14-8\\
-5+0+42&6+0+28&10+0+14
\end{array}
\right)\\
&=\left(
\begin{array}{ccc}
-2&29&-45\\
-28&6&-2\\
37&34&24
\end{array}
\right)
\end{align*}
\\
\begin{align*}
\hat N\hat M
&=\left(
\begin{array}{ccc}
-5+12+10&-35+12+0&15-24+70\\
3+10-7&21+10+0&-9-20-49\\
6+8+2&42+8+0&-18-16+14
\end{array}
\right)\\
&=\left(
\begin{array}{ccc}
17&-23&61\\
6&31&-78\\
16&50&-20
\end{array}
\right)
\end{align*}
\section*{Vector Multiplication}
\[
\vec{u}^T\vec{v}=-6+0-4=-10
\]
\[
\vec{u}\vec{v}^T=\left(
\begin{array}{ccc}
-6&0&3\\
4&0&-2\\
8&0&-4
\end{array}
\right)
\]
\section*{Plane}
Assume the equation of this plane is $f(x,y,z)=Ax+By+Cz+D=0$. We have
\[
\left\{
\begin{array}{ccc}
A+2B+3C+D=0\\
3A-2B+7C+D=0\\
-2A-2B+4C+D=0
\end{array}
\right.
\]
Solving these equations we can get 
\[
A=-\frac{3}{5}C, B=\frac{7}{10}C,D=-\frac{19}{5}C
\]
So the equation of this plane is $f(x,y,z)=6x-7y-10z+38=0$
\end{document}